Since I've advocated not memorizing the quotient rule, I'll do this one from first principles,
using the product rule.
\begin{align*}
  \frac{\der}{\der \theta}& \tan\theta \\
        &=   \frac{\der}{\der \theta}\left(\frac{\sin\theta}{\cos\theta}\right) \\
        &=   \frac{\der}{\der \theta}\left[\sin\theta\left(\cos\theta\right)^{-1}\right] \\
        &=   \cos\theta\left(\cos\theta\right)^{-1}+(\sin\theta)(-1)(\cos\theta)^{-2}(-\sin\theta)\\
        &=   1+\tan^2\theta
\end{align*}
(Using a trig identity, this can also be rewritten as $\sec^2\theta$.)
